Complete traversal function
Added triggers to size, needed more cases in previous lemmas
Need to clean up code, maybe prove induction principle

src/core/TermFuncs.v
@@ -1676,7 +1676,7 @@ Fixpoint term_size (t: term_c) : nat :=
   | Tlet t1 (_, _, t2) => 1 + term_size t1 + term_size t2
   | Tcase t1 pats => 1 + term_size t1 + sum (map (fun x => term_size (snd x)) pats)
   | Teps (_, _, t) => 1 + term_size t
-  | Tquant _ (_, _, _, t) => 1 + term_size t
+  | Tquant _ (_, _, tr, t) => 1 + term_size t + sum (map (fun l => sum (map term_size l)) tr) 
   | Tbinop _ t1 t2 => 1 + term_size t1 + term_size t2
   | Tnot t => 1 + term_size t
   | Ttrue => 1
@@ -1692,7 +1692,7 @@ Definition term_node_size (t: term_node) : nat :=
   | Tlet t1 (_, _, t2) => 1 + term_size t1 + term_size t2
   | Tcase t1 pats => 1 + term_size t1 + sum (map (fun x => term_size (snd x)) pats)
   | Teps (_, _, t) => 1 + term_size t
-  | Tquant _ (_, _, _, t) => 1 + term_size t
+  | Tquant _ (_, _, tr, t) => 1 + term_size t + sum (map (fun l => sum (map term_size l)) tr) 
   | Tbinop _ t1 t2 => 1 + term_size t1 + term_size t2
   | Tnot t => 1 + term_size t
   | Ttrue => 1
@@ -1704,6 +1704,16 @@ Proof. destruct tm; reflexivity. Qed.
 
 (*This will be generic for any errState (CoqBigInt.t * St) for some state St.
   This is the most generic we will need for our purposes*)
+(*This is similar to [t_map] in the OCaml version, with 1 big difference:
+  t_map is not explicitly recursive. However, it can be used recursively by instantiating
+  the function argument with a recursive function. This doesn't work for us because Coq would
+  not be able to prove such a function terminating.
+  So instead we give a generic recursive traversal function that opens all the bindings.
+  Defining this is extremely complicated. The recursion is not structural (since we do substitution
+  when opening bindings). So we give a size metric and prove that substitution of variables
+  preserves size (which is not trivial). Then, since we need to make recursive calls inside state
+  monad bind operations, we need a dependently typed bind operator to remember the hypotheses
+  we need. For similar reasons, we also need a dependently typed [map] function on lists*)
 Section Traverse.
 (*NOT dependently typed for OCaml purposes*)
 Variable (St: Type). (*The type of state*)
@@ -1722,8 +1732,14 @@ Variable (if_case: forall (t1 t2 t3: term_c) (r1 r2 r3: R), T).
 Variable (app_case: forall (l: lsymbol) (tms: list term_c) (rs: list R), T).
 (*Again, tbs is a list of (new pattern, new term, recursive call)*)
 Variable (match_case: forall (t1: term_c) (r1: R) (tb: list (pattern_c * term_c * R)), T).
-
-Variable (evil: forall (t: term_c), T).
+(*As above: new variable, new term, new result*)
+Variable (eps_case: forall (v: vsymbol) (t: term_c) (r: R), T).
+Variable (quant_case: forall (q: quant) (vs: list vsymbol) (tr: list (list (term_c))) (rr: list (list R))
+  (t: term_c) (r: R), T).
+Variable (binop_case: forall (b: binop) (t1 t2: term_c) (r1 r2: R), T).
+Variable (not_case: forall (t: term_c) (r: R), T).
+Variable (true_case: T).
+Variable (false_case : T).
 
 (*This is annoying for sure*)
 
@@ -1778,7 +1794,8 @@ Fixpoint t_shape (t1 t2: term_c) {struct t1} : bool :=
    forallb (fun x => x) (Common.map2 (fun x y => t_shape (snd x) (snd y)) b1 b2)
   | Teps (_, _, t1), Teps (_, _, t2) => t_shape t1 t2
   | Tquant q1 (_, _, tr1, t1), Tquant q2 (_, _, tr2, t2) => quant_eqb q1 q2 && 
-    t_shape t1 t2
+    t_shape t1 t2 && (length tr1 =? length tr2) &&
+      all2 (fun x y => length x =? length y) tr1 tr2 && all2 (all2 t_shape) tr1 tr2
   | Tbinop b1 t1 t2, Tbinop b2 t3 t4 => binop_eqb b1 b2 && t_shape t1 t3 && t_shape t2 t4
   | Tnot t1, Tnot t2 => t_shape t1 t2
   | Ttrue, Ttrue => true
@@ -1876,13 +1893,15 @@ Qed.
 Lemma t_shape_quant {t1 t2 q vs1 b1 tr1 tm1}:
   t_shape t1 t2 ->
   t_node_of t1 = Tquant q (vs1, b1, tr1, tm1) ->
-  exists vs2 b2 tr2 tm2, t_node_of t2 = Tquant q (vs2, b2, tr2, tm2) /\ t_shape tm1 tm2.
+  exists vs2 b2 tr2 tm2, t_node_of t2 = Tquant q (vs2, b2, tr2, tm2) /\ t_shape tm1 tm2 /\
+  length tr1 = length tr2 /\ all2 (fun x y => length x =? length y) tr1 tr2 /\ 
+  all2 (all2 t_shape) tr1 tr2.
 Proof.
   intros Hshape Heq. 
   destruct t1 as [n1 ? ? ?]; destruct t2 as [n2 ? ? ?]; destruct n1; try solve[inversion Heq].
   simpl in Hshape. destruct p as [[[vs2 b2] tr2] e2]. destruct n2; try solve[inversion Hshape].
   destruct p as [[[vs3 b3] tr3] e3]. simpl in Heq. inversion Heq; subst; clear Heq.
-  bool_hyps. apply quant_eqb_eq in H. subst. simpl. repeat eexists; eauto.
+  bool_hyps. apply quant_eqb_eq in H. subst. apply Nat.eqb_eq in H2. simpl. repeat eexists; eauto.
 Qed.
 
 Lemma t_shape_binop {t1 t2 b tm1 tm2}:
@@ -1952,8 +1971,22 @@ Proof.
     intros Hlen. rewrite all2_cons. intros Hall. bool_hyps. inversion H0; subst; f_equal; eauto.
   - destruct (t_shape_eps Hshape Heq) as [v2 [b2 [e2 [Heq2 Hshape2]]]].
     rewrite !term_size_eq, Heq, Heq2; simpl. eauto.
-  - destruct (t_shape_quant Hshape Heq) as [vs2 [b2 [tr2 [tm2 [Heq2 Hshape2]]]]].
-    rewrite !term_size_eq, Heq, Heq2. simpl. auto.
+  - destruct (t_shape_quant Hshape Heq) as [vs2 [b2 [tr2 [tm2 [Heq2 [Hshape2 [Hlen [Htrlen Htrs]]]]]]]].
+    rewrite !term_size_eq, Heq, Heq2. simpl. f_equal. f_equal; auto.
+    f_equal. clear -Hlen Htrs Htrlen H.
+    generalize dependent tr2. induction tr as [| h1 t1 IH]; simpl; auto;
+    intros [| h2 t2]; try discriminate; auto.
+    simpl. intros Hlen. rewrite !all2_cons. intros Halllen Hall. 
+    apply andb_true_iff in Halllen, Hall. destruct Hall as [Hshapeh Hshapet].
+    destruct Halllen as [Hlenh Hlent].
+    inversion H; subst.
+    f_equal; auto.
+    clear -H2 Hshapeh Hlenh.
+    (*TODO: should have better way to do this*)
+    generalize dependent h2.
+    induction h1 as [| x1 t1 IH]; intros [| x2 t2]; simpl; auto; try discriminate.
+    intros Hlen. rewrite all2_cons. intros Hall. apply andb_true_iff in Hall; destruct Hall
+    as [Hshapex Hshapet]; inversion H2; subst; f_equal; auto.
   - destruct (t_shape_binop Hshape Heq) as [e1 [e2 [Heq2 [Hshape1 Hshape2]]]].
     rewrite !term_size_eq, Heq, Heq2; simpl; auto.
   - destruct (t_shape_not Hshape Heq) as [tm2 [Heq2 Hshape2]];
@@ -1961,6 +1994,14 @@ Proof.
   - rewrite !term_size_eq, Ht, (t_shape_true Hshape Ht). reflexivity.
   - rewrite !term_size_eq, Ht, (t_shape_false Hshape Ht). reflexivity.
 Qed. 
+
+Lemma all2_len_eq {A: Type} (l: list (list A)):
+  all2 (fun x y => length x =? length y) l l.
+Proof.
+  induction l as [| h t IH]; simpl; auto.
+  rewrite all2_cons; apply andb_true_iff; split; auto.
+  rewrite Nat.eqb_refl; auto.
+Qed.
 
 Lemma t_shape_refl t:
   t_shape t t.
@@ -1975,7 +2016,14 @@ Proof.
   - rewrite Nat.eqb_refl. solve_bool. apply andb_true_iff; split; auto.
     induction tbs as [| h1 tl1 IH]; simpl; auto.
     inversion H0; subst; apply andb_true_iff; split; auto.
-  - apply andb_true_iff; split; auto. apply quant_eqb_eq; auto.
+  - unfold is_true. rewrite !andb_true_iff; split_all; auto.
+    + apply quant_eqb_eq; auto.
+    + rewrite Nat.eqb_refl; auto.
+    + apply all2_len_eq. 
+    + clear -H. induction tr as [| h t IH]; auto. rewrite all2_cons. inversion H; subst.
+      apply andb_true_iff; split; auto. clear -H2.
+      induction h as [| h t IH]; simpl; auto. rewrite all2_cons. inversion H2; subst.
+      apply andb_true_iff; split; auto.
   - unfold is_true; rewrite !andb_true_iff; split_all; auto.
     apply binop_eqb_eq; auto.
 Qed. 
@@ -1985,6 +2033,13 @@ Lemma all2_shape_refl l:
 Proof.
   induction l as [| h1 t1 IH]; auto.
   rewrite all2_cons, t_shape_refl; auto.
+Qed.
+
+Lemma all2_all2_shape_refl l:
+  all2 (all2 t_shape) l l.
+Proof.
+  induction l as [| h1 t1 IH]; auto.
+  rewrite all2_cons, all2_shape_refl. auto.
 Qed.
 
 Lemma t_shape_node t1 t2:
@@ -2000,7 +2055,8 @@ Proof.
   - simpl. rewrite Nat.eqb_refl. simpl. clear -H0. induction tbs as [| h2 tl2 IH]; simpl; auto.
     inversion H0; subst.
     rewrite t_shape_refl; auto.
-  - rewrite andb_true_r. apply quant_eqb_eq; auto.
+  - rewrite Nat.eqb_refl, all2_len_eq, all2_all2_shape_refl, !andb_true_r.
+    apply quant_eqb_eq; auto.
   - rewrite !andb_true_r. apply binop_eqb_eq; auto. 
 Qed.
 
@@ -2031,7 +2087,8 @@ Proof.
   - intros Heq. apply term_bound_eqb_eq in Heq; subst.
     destruct p0 as [[v2 b2] t2]; apply t_shape_refl.
   - intros [Heq1 Heq2]. apply term_quant_eqb_eq in Heq2. subst.
-    destruct p0 as [[[vs1 b1] tr1] t1]; apply andb_true_iff; split;auto; apply t_shape_refl.
+    destruct p0 as [[[vs1 b1] tr1] t1].
+    rewrite t_shape_refl, Nat.eqb_refl, all2_len_eq, all2_all2_shape_refl, !andb_true_r; auto.
   - intros [[Heq1 Heq2] Heq3].
     apply term_eqb_eq in Heq2, Heq3. subst. rewrite !t_shape_refl. split_all; auto.
   - intros Heq. apply term_eqb_eq in Heq; subst; apply t_shape_refl.
@@ -2136,7 +2193,17 @@ Proof.
     rewrite (term_size_eq tm2), t_subst_unsafe_aux_rewrite, Heq.
     simpl. rewrite term_size_attr_copy. simpl. f_equal.
     destruct (Mvs.is_empty _); auto.
-    apply IH2, subst_vars_ok2; auto.
+    + f_equal; auto. f_equal.
+      clear -IH1 Hm1. induction tr as [| l1 t1 IH]; simpl; auto.
+      inversion IH1; subst. f_equal; auto.
+      clear -H1 Hm1. induction l1 as [| h1 t1 IH]; simpl; auto.
+      inversion H1; subst; auto.
+    + f_equal.
+      * apply IH2, subst_vars_ok2; auto.
+      * f_equal. clear -IH1 Hm1. induction tr as [| l1 t1 IH]; simpl; auto.
+        inversion IH1; subst. f_equal; auto.
+        clear -H1 Hm1. induction l1 as [| h1 t1 IH]; simpl; auto.
+        inversion H1; subst; auto.
   - (*binop*) intros b t1 t2 tm2 Heq IH1 IH2 m1 Hm1.
     rewrite (term_size_eq tm2), t_subst_unsafe_aux_rewrite, Heq.
     unfold t_map_unsafe. rewrite term_size_attr_copy, Heq. simpl.
@@ -2176,14 +2243,13 @@ Proof.
 Qed.
 
 (*Interesting case - why we need dependent bind*)
-Lemma tlet_size2 {t1 b y s tm}
-(Hsz: term_node_size (Tlet t1 b) = term_size tm)
+Lemma dep_bnd_size_bound {b y s}
 (Heq : forall z : vsymbol * term_c,
   fst
   (run_errState
   (@errst_tup1 CoqBigInt.t St _ (errst_lift1 (t_open_bound b))) s) =
   inr z -> y = z):
-  term_size (snd y) < term_size tm.
+term_size (snd y) = term_size (snd b).
 Proof.
   unfold errst_tup1 in Heq. Opaque t_open_bound. simpl in Heq.
   unfold run_errState in Heq. simpl in Heq.
@@ -2193,8 +2259,64 @@ Proof.
   (*Now we just need to reason about [t_open_bound] and its size*)
   pose proof (t_open_bound_size b (fst s)) as Hszb.
   rewrite Hrun in Hszb. simpl in Hszb.
-  rewrite Hszb. 
-  (*And now return to main obligation*)
+  auto.
+Qed.
+
+(*And the branch version*)
+
+Lemma t_open_branch_size (b: term_branch): forall s,
+  term_size (snd (fst (runState (t_open_branch b) s))) = term_size (snd b).
+Proof.
+  intros s. destruct b as [[v b] t].
+  Opaque pat_rename.
+  simpl.
+  destruct (runState (pat_rename Mvs.empty v) s) as [[m1 v1] s1] eqn : Hrun.
+  simpl.
+  (*Get m1 value*)
+  Transparent pat_rename. Opaque add_vars.
+  simpl in Hrun.
+  destruct (runState (add_vars (Svs.elements (pat_vars_of v))) s) as [v3 s3] eqn : Hrun3.
+  inversion Hrun; subst.
+  (*We don't care that the variable is fresh, but we care that it is a variable*)
+  apply t_subst_unsafe_size.
+  intros v2 tm1. rewrite Mvs.union_spec; auto.
+  rewrite Mvs.empty_spec.
+  destruct (Mvs.find_opt v2 (Mvs.map t_var v3)) as [l2|] eqn : Hfind; [|discriminate].
+  intros Hsome; inversion Hsome; subst.
+  apply Mvs.map_spec in Hfind.
+  destruct Hfind as [k1 [v1 [Heqv [Hfind Htm1]]]]; subst.
+  reflexivity.
+Qed.
+
+Lemma dep_bnd_size_branch {b y s}
+(Heq: forall z : pattern_c * term_c,
+    fst
+    (run_errState
+    (@errst_tup1 CoqBigInt.t St _ (errst_lift1 (t_open_branch b))) s) =
+    inr z -> y = z):
+term_size (snd y) = term_size (snd b).
+Proof.
+  unfold errst_tup1 in Heq. Opaque t_open_branch. simpl in Heq.
+  unfold run_errState in Heq. simpl in Heq.
+  destruct (runState (t_open_branch b) (fst s)) as [v1 s1] eqn : Hrun.
+  simpl in Heq.
+  specialize (Heq v1 eq_refl). subst.
+  pose proof (t_open_branch_size b (fst s)) as Hszb.
+  rewrite Hrun in Hszb. simpl in Hszb. auto.
+Qed.
+
+(*Back to lemmas*)
+
+Lemma tlet_size2 {t1 b y s tm}
+(Hsz: term_node_size (Tlet t1 b) = term_size tm)
+(Heq : forall z : vsymbol * term_c,
+  fst
+  (run_errState
+  (@errst_tup1 CoqBigInt.t St _ (errst_lift1 (t_open_bound b))) s) =
+  inr z -> y = z):
+  term_size (snd y) < term_size tm.
+Proof.
+  rewrite (dep_bnd_size_bound Heq).
   simpl in Hsz. destruct b as [[b1 b2] b3]; simpl. lia.
 Qed.
 
@@ -2227,29 +2349,6 @@ Qed.
 
 (*Interesting case for match*)
 
-Lemma t_open_branch_size (b: term_branch): forall s,
-  term_size (snd (fst (runState (t_open_branch b) s))) = term_size (snd b).
-Proof.
-  intros s. destruct b as [[v b] t].
-  Opaque pat_rename.
-  simpl.
-  destruct (runState (pat_rename Mvs.empty v) s) as [[m1 v1] s1] eqn : Hrun.
-  simpl.
-  (*Get m1 value*)
-  Transparent pat_rename. Opaque add_vars.
-  simpl in Hrun.
-  destruct (runState (add_vars (Svs.elements (pat_vars_of v))) s) as [v3 s3] eqn : Hrun3.
-  inversion Hrun; subst.
-  (*We don't care that the variable is fresh, but we care that it is a variable*)
-  apply t_subst_unsafe_size.
-  intros v2 tm1. rewrite Mvs.union_spec; auto.
-  rewrite Mvs.empty_spec.
-  destruct (Mvs.find_opt v2 (Mvs.map t_var v3)) as [l2|] eqn : Hfind; [|discriminate].
-  intros Hsome; inversion Hsome; subst.
-  apply Mvs.map_spec in Hfind.
-  destruct Hfind as [k1 [v1 [Heqv [Hfind Htm1]]]]; subst.
-  reflexivity.
-Qed.
 
 Lemma tmatch_size2 {tm1 s y b}
   (Hx: term_size (snd b) < term_size tm1)
@@ -2261,16 +2360,8 @@ Lemma tmatch_size2 {tm1 s y b}
     inr z -> y = z):
   term_size (snd y) < term_size tm1.
 Proof.
-  unfold errst_tup1 in Heq. Opaque t_open_branch. simpl in Heq.
-  unfold run_errState in Heq. simpl in Heq.
-  destruct (runState (t_open_branch b) (fst s)) as [v1 s1] eqn : Hrun.
-  simpl in Heq.
-  specialize (Heq v1 eq_refl). subst.
-  (*Now we just need to reason about [t_open_bound] and its size*)
-  pose proof (t_open_branch_size b (fst s)) as Hszb.
-  rewrite Hrun in Hszb. simpl in Hszb.
-  rewrite Hszb. auto.
-Qed. 
+  rewrite (dep_bnd_size_branch Heq). auto.
+Qed.
 
 Lemma tmatch_size3 {tm1 t1 tbs}
   (Hsz: term_node_size (Tcase t1 tbs) = term_size tm1):
@@ -2290,7 +2381,156 @@ Proof.
   simpl in Hsz. lia.
 Qed.
 
+Lemma teps_size {b y s tm}
+(Hsz: term_node_size (Teps b) = term_size tm)
+(Heq : forall z : vsymbol * term_c,
+  fst
+  (run_errState
+  (@errst_tup1 CoqBigInt.t St _ (errst_lift1 (t_open_bound b))) s) =
+  inr z -> y = z):
+  term_size (snd y) < term_size tm.
+Proof.
+  rewrite (dep_bnd_size_bound Heq). simpl in Hsz. destruct b as [[b1 b2] b3]; simpl in Hsz. 
+  simpl. lia.
+Qed.
 
+(*Do this separately because we need induction*)
+Lemma vl_rename_aux_map vs s (m: Mvs.t term_c) x 
+  (Hm: forall k t, Mvs.find_opt k m = Some t -> term_size t = 1):
+  forall k t, Mvs.find_opt k (fst (fst (runState (vl_rename_aux vs (st_ret (m , x))) s))) = Some t -> 
+  term_size t = 1.
+Proof.
+  revert s m x Hm. induction vs as [| h1 t1 IH]; simpl; auto.
+  intros s m x Hm k t.
+  destruct (runState (fresh_vsymbol h1) s ) as [v1 s1] eqn : Hrun1; simpl.
+  destruct (runState _ s1) as [v2 s2] eqn : Hrun2; simpl.
+  replace v2 with (fst (runState
+      (vl_rename_aux t1 (st_ret (Mvs.add h1 (t_var v1) m, v1 :: x))) s1)) by (rewrite Hrun2; auto).
+  apply IH. intros k1 tm1. rewrite Mvs.add_spec.
+  destruct (Vsym.Tg.equal k1 h1); auto; [| apply Hm].
+  intros Hsome; inversion Hsome; subst; reflexivity.
+Qed.
+
+Lemma t_open_quant1_size (b: term_quant): forall s,
+  term_size (snd (fst (runState (t_open_quant1 b) s))) = term_size (snd b) /\
+  Forall2 (Forall2 (fun x y => term_size x = term_size y)) (snd (fst (fst (runState (t_open_quant1 b) s)))) (snd (fst b)).
+Proof.
+  intros s. destruct b as [[[vs b] tr] t].
+  Opaque vl_rename.
+  simpl.
+  destruct (runState (vl_rename Mvs.empty vs) s) as [[m1 v1] s1] eqn : Hrun.
+  simpl.
+  (*Get m1 value*)
+  Transparent vl_rename. Opaque vl_rename_aux. simpl in Hrun.
+  destruct (runState (vl_rename_aux vs (st_ret (Mvs.empty, []))) s) as [v3 s3] eqn : Hrun3.
+  simpl in Hrun3. inversion Hrun; subst.
+  replace v3 with (fst (runState (vl_rename_aux vs (st_ret (Mvs.empty, []))) s)) by (rewrite Hrun3; auto).
+  split.
+  - apply t_subst_unsafe_size. apply vl_rename_aux_map. intros k1 v1. rewrite Mvs.empty_spec. discriminate.
+  - induction tr as [|tr1 tr2 IH]; auto.
+    constructor; auto.
+    induction tr1 as [| tm1 tm2 IH1]; auto.
+    constructor; auto.
+    apply t_subst_unsafe_size, vl_rename_aux_map. intros k1 v1. rewrite Mvs.empty_spec. discriminate.
+Qed.
+
+Lemma dep_bnd_size_quant {b y s}
+(Heq : forall z : list vsymbol * trigger * term_c,
+fst
+(run_errState
+(@errst_tup1 CoqBigInt.t St _ (errst_lift1 (t_open_quant1 b)))
+s) = inr z -> y = z):
+(*Here we need info both about term and triggers*)
+term_size (snd y) = term_size (snd b) /\
+Forall2 (Forall2 (fun x y => term_size x = term_size y)) (snd (fst y)) (snd (fst b)). 
+Proof.
+  unfold errst_tup1 in Heq. Opaque t_open_quant1. simpl in Heq.
+  unfold run_errState in Heq. simpl in Heq.
+  destruct (runState (t_open_quant1 b) (fst s)) as [v1 s1] eqn : Hrun.
+  simpl in Heq.
+  specialize (Heq v1 eq_refl). subst.
+  (*Now we just need to reason about [t_open_quant1] and its size*)
+  pose proof (t_open_quant1_size b (fst s)) as Hszb.
+  rewrite Hrun in Hszb. simpl in Hszb. auto.
+Qed.
+
+Lemma tquant_size_tr {q tq s y tm1}
+  (Hsz: term_node_size (Tquant q tq) = term_size tm1)
+  (Heq: forall z : list vsymbol * trigger * term_c,
+    fst
+    (run_errState
+    (@errst_tup1 CoqBigInt.t St _ (errst_lift1 (t_open_quant1 tq)))
+    s) = inr z -> y = z):
+  Forall (Forall (fun x : term_c => term_size x < term_size tm1)) (snd (fst y)).
+Proof.
+  pose proof (dep_bnd_size_quant Heq) as [Hsz1 Hsz2].
+  simpl in Hsz. clear Heq. destruct tq as [[[vs b] tr] t]; simpl in *.
+  assert (Hsz': sum (map (fun l => sum (map term_size l)) tr) < term_size tm1) by lia.
+  clear -Hsz' Hsz2.
+  generalize dependent tr. induction (snd (fst y)) as [| h1 t1 IH]; simpl; 
+  intros [| h2 t2]; simpl; auto; intros Hall; inversion Hall; subst.
+  intros Hsz. constructor; auto. 2: eapply IH; eauto; lia.
+  assert (Hh2: sum (map term_size h2) < term_size tm1) by lia.
+  clear -Hh2 H2. generalize dependent h2.
+  induction h1 as [| x1 t1 IH]; intros [| x2 t2]; simpl; auto; intros Hall;
+  inversion Hall; subst; auto. intros Hsz. constructor; auto; try lia.
+  eapply IH; eauto; lia.
+Qed.
+
+Lemma tquant_size1 {q tq s y tm1}
+  (Hsz: term_node_size (Tquant q tq) = term_size tm1)
+  (Heq: forall z : list vsymbol * trigger * term_c,
+    fst
+    (run_errState
+    (@errst_tup1 CoqBigInt.t St _ (errst_lift1 (t_open_quant1 tq)))
+    s) = inr z -> y = z):
+  term_size (snd y) < term_size tm1.
+Proof.
+  pose proof (dep_bnd_size_quant Heq) as [Hsz1 Hsz2]. rewrite Hsz1.
+  simpl in Hsz. destruct tq as [[[vs b] tr] t]; simpl in *. lia.
+Qed.
+
+Lemma tbinop_size1 {b t1 t2 tm}
+  (Hsz : term_node_size (Tbinop b t1 t2) = term_size tm):
+  term_size t1 < term_size tm.
+Proof.
+  simpl in Hsz. lia.
+Qed.
+
+Lemma tbinop_size2 {b t1 t2 tm}
+  (Hsz : term_node_size (Tbinop b t1 t2) = term_size tm):
+  term_size t2 < term_size tm.
+Proof.
+  simpl in Hsz. lia.
+Qed.
+
+Lemma tnot_size1 {t1 tm}
+  (Hsz : term_node_size (Tnot t1) = term_size tm):
+  term_size t1 < term_size tm.
+Proof.
+  simpl in Hsz. lia.
+Qed.
+
+
+
+(*Lemma dep_bnd_size_bound {b y s}
+(Heq : forall z : vsymbol * term_c,
+  fst
+  (run_errState
+  (@errst_tup1 CoqBigInt.t St _ (errst_lift1 (t_open_bound b))) s) =
+  inr z -> y = z):
+term_size (snd y) = term_size (snd b).
+Proof.
+  unfold errst_tup1 in Heq. Opaque t_open_bound. simpl in Heq.
+  unfold run_errState in Heq. simpl in Heq.
+  destruct (runState (t_open_bound b) (fst s)) as [v1 s1] eqn : Hrun.
+  simpl in Heq.
+  specialize (Heq v1 eq_refl). subst.
+  (*Now we just need to reason about [t_open_bound] and its size*)
+  pose proof (t_open_bound_size b (fst s)) as Hszb.
+  rewrite Hrun in Hszb. simpl in Hszb.
+  auto.
+Qed.*)
 
 (*TODO: move from IndProp*)
 
@@ -2301,8 +2541,6 @@ Fixpoint dep_map {A B: Type} {P: A -> Prop} (f: forall x, P x -> B)
   | x :: tl => fun Hforall => f x (Forall_inv Hforall) ::
     dep_map f tl (Forall_inv_tail Hforall)
   end Hall.
-
-Print term_c.
 
 Fixpoint term_traverse (tm1: term_c) (ACC: Acc lt (term_size tm1)) : T :=
   match (t_node_of tm1) as t1 return term_node_size t1 = term_size tm1 -> _ with
@@ -2338,10 +2576,37 @@ Fixpoint term_traverse (tm1: term_c) (ACC: Acc lt (term_size tm1)) : T :=
             errst_ret (y, t2))
         ) tbs (tmatch_size3 Hsz)) ;;
     match_case t1 r1 tbs2
-
-
-  | _ => fun Hsz => evil tm1
+  | Teps b => fun Hsz =>
+    errst_bind_dep' (errst_tup1 (errst_lift1 (t_open_bound b)))
+      (fun y s Heq => 
+        v <- (term_traverse (snd y) (Acc_inv ACC (teps_size Hsz Heq))) ;;
+        eps_case (fst y) (snd y) v)
+  (*A slight complication from the triggers - need nested dependent match*)
+  | Tquant q tq => fun Hsz =>
+    (*NOTE: doing bind ... ret, need for proofs even though superflous*)
+    errst_bind_dep' (errst_tup1 (errst_lift1 (t_open_quant1 tq)))
+      (fun (y : list vsymbol * trigger * term_c) s Heq => 
+        v <- (term_traverse (snd y) (Acc_inv ACC (tquant_size1 Hsz Heq))) ;;
+        let vs := fst (fst y) in
+        let tr := snd (fst y) in
+        let t := snd y in
+        (*Then traverse over triggers*)
+        v2 <- errst_list (dep_map (fun l1 (Hl1: Forall (fun x => term_size x < term_size tm1) l1) =>
+          errst_list (dep_map (fun tr1 (Ht1: term_size tr1 < term_size tm1) => 
+            term_traverse tr1 (Acc_inv ACC Ht1))
+            l1 Hl1)) tr (tquant_size_tr Hsz Heq)) ;;
+        quant_case q vs tr v2 t v)
+  | Tbinop b t1 t2 => fun Hsz =>
+    r1 <- term_traverse t1 (Acc_inv ACC (tbinop_size1 Hsz)) ;;
+    r2 <- term_traverse t2 (Acc_inv ACC (tbinop_size2 Hsz)) ;;
+    binop_case b t1 t1 r1 r2
+  | Tnot t1 => fun Hsz =>
+    r1 <- term_traverse t1 (Acc_inv ACC (tnot_size1 Hsz)) ;;
+    not_case t1 r1
+  | Ttrue => fun _ => true_case
+  | Tfalse => fun _ => false_case
   end (eq_sym (term_size_eq tm1)).
+
 (* 
 Equations term_traverse (tm1: term_c) : T by wf (term_size tm1) lt :=
   term_traverse tm1 := term_node_traverse (t_node_of tm1) 
